examples/unit-tests/mac.fst
@@ -14,7 +14,7 @@
    limitations under the License.
 *)
 
-module MacIdeal 
+module MAC 
 open Array
 type bytes    = seq byte
 type text     = bytes
@@ -25,21 +25,33 @@ let macsize = 20
 type key = nbytes keysize
 type tag = nbytes macsize
 
-(* we rely on some external crypto library for SHA1 *)
+(* we rely on some external crypto library implementing HMAC-SHA1 *)
 
 assume val sha1: key -> text -> Tot tag 
+val sha1verify: key -> text -> tag -> Tot bool
+let sha1verify k txt tag = (sha1 k txt = tag)
 
-(* TODO make keys abstract *) 
-
-(* we attach authenticated properties to keys *) 
+(* we attach an authenticated properties to each key *) 
 
 opaque type key_prop : key -> text -> Type
 type pkey (p:(text -> Type)) = k:key{key_prop k == p}
 
-assume val new_key: p:(text -> Type) -> pkey p
+assume val keygen: p:(text -> Type) -> pkey p
 
+(* TODO make keys abstract except within this module *) 
 
 (* to model authentication, we log all genuine calls to MACs *) 
+
+val mac:    k:key -> t:text{key_prop k t} -> tag
+val verify: k:key -> t:text -> tag -> b:bool{b ==> key_prop k t}
+
+
+
+(* the ideal implementation below uses a global log *)
+
+(* TODO provide a concrete implementation of keygen, aka sample 16
+   random bytes + maybe a counter it would be better to avoid assuming
+   key_prop; see also encrypt.fst *)
 
 type entry = 
   | Entry : k:key
@@ -47,21 +59,21 @@ type entry =
          -> m:tag
          -> entry
 
+(* TODO why assumed? we miss toplevel side effects... *) 
+
 assume val log : ref (list entry)
 
-val mac: k:key
-      -> t:text{key_prop k t}
-      -> tag
 let mac k t = 
   let m = sha1 k t in
   log := Entry k t m :: !log;
   m
 
-val verify: k:key
-         -> t:text 
-         -> tag 
-         -> b:bool{b ==> key_prop k t}
-let verify k t m = 
-  let found = List.find (function (Entry k' t' _) -> k=k' && t=t') !log in
-  is_Some found
+let verify k text tag = 
+  let verified = sha1verify k text tag in 
+  let found    = is_Some(List.find (function (Entry k' text' tag') -> k=k' && text=text' (*CTXT: && tag=tag' *) ) !log) in 
+//verified           (* concrete: we never read the log *) 
+  verified && found  (* ideal: we correct errors. *)
+//(if verified && not found then winner:= Some(k,text,tag)) verified (* winning condition against for INT-CPA *)
 
+(* VARIANT CTXT vs CPA: is the tag authenticated? 
+   otherwise do not include m:tag in the entry *)
