examples/unit-tests/rpc.fst
@@ -1,16 +1,22 @@
 (* Copyright (c) Microsoft Corporation.  All rights reserved.  *)
+
 module RPC
-open MacIdeal
-open Format
 open Array
+open Format
+open MAC
+
+(* some basic, untrusted network controlled by the adversary *)
 
 assume val send: message -> unit
 assume val recv: (message -> unit) -> unit
+
+(* two events, recording genuine requests and responses *)
+
 logic type Request : string -> Type
 logic type Response : string -> string -> Type
 
-(* let k = new_key (fun msg -> (exists s. msg = request s /\ Request s) \/       *)
-(*                             (exists s t. msg = response s t /\ Response s t)) *)
+(* let k = keygen (fun msg -> (exists s. msg = request s /\ Request s) \/       *)
+(*                            (exists s t. msg = response s t /\ Response s t)) *)
 opaque logic type reqresp (msg:message) =
     (exists s. msg = request s /\ Request s)
       \/ (exists s t. msg = response s t /\ Response s t)
@@ -21,8 +27,7 @@ let client (s:string16) =
   assume (Request s);
   send (append (utf8 s) (mac k (request s))); 
   recv (fun msg ->
-    if length msg < macsize
-    then failwith "Too short"
+    if length msg < macsize then failwith "Too short"
     else
       let (v, m') = split msg (length msg - macsize) in
       let t = iutf8 v in
@@ -31,16 +36,17 @@ let client (s:string16) =
 
 let server () =
   recv (fun msg ->
-    if length msg < macsize
-    then failwith "Too short"
+    if length msg < macsize then failwith "Too short"
     else
       let (v,m) = split msg (length msg - macsize) in
-      let s = iutf8 v in
-      if verify k (request s) m && length v < 65536 //NEEDED THIS CHECK to make a well-formed response
-      then  (assert (Request s);
-             let t = "22" in
-             assume (Response s t);
-             send (append (utf8 t) (mac k (response s t)))))
+      if length v > 65535 then failwith "Too long" // we need this check to ensure a well-formed response
+      else
+        let s = iutf8 v in
+        if verify k (request s) m 
+        then  
+          ( assert (Request s);
+            let t = "22" in
+            assume (Response s t);
+            send (append (utf8 t) (mac k (response s t)))))
     
-
 (* let test () = server(); client "2 + 2?" *)
